reordanize file structure

Stlc/Classes.v
@@ -6,16 +6,56 @@ From Equations Require Import Equations.
 (** * Operations *)
 (***********************************************************************)
 
+(* Syntactic operations on terms of type `e n`, i.e. those that contain 
+   at most `n` bound variables. We call `n` the "scope index" --- number 
+   of bound variables that are in scope. (The set of allowed free variables
+   is not tracked by the type system.)
+*)
+   
+
 Class Syntax (e : nat -> Set) := {
+
+    (* List free variables *)
     fv : forall {n}, e n -> vars ;
+
+    (* Count number of nodes in AST *)
     size : forall {n}, e n -> nat ;
+
+    (* Increase the scope index, but do not modify the term *)
     weaken : forall {n}, e n -> e (S n) ;
-    close : forall {n}, atom -> e n -> e (S n) ;
+
+    (* Replace the given free variable with bound variable `n`, increasing
+       the scope of the term. *)
+    close : forall {n}, var -> e n -> e (S n) ;
 }.
 
+
+(* Substitution operations.  
+
+   This class is indexed by two types so that it can include, for example,
+   substituting types in terms as well as substituting terms in terms. 
+   This is more general than needed for STLC, but adds flexibility to 
+   the overall approach.
+
+*)
+
 Class Subst (e : nat -> Set) (u : nat -> Set) `{Syntax e} `{Syntax u} := {
+
+    (* bound variable substitution
+
+       Replaces bound variable n with a term of type `u n` inside a 
+       term of type `e (S n)`. Because we are replacing the largest index
+       we can decrement the scope.
+     *)
     open  : forall {n}, u n -> e (S n) -> e n ;
-    subst : forall {n}, u n -> atom -> e n -> e n    
+
+    (* free variable substitution
+
+       Replaces free variable by term of type `u n` in an expression
+       of type `e n`. Doesn't change the scoping of bound variables.
+     *)
+
+    subst : forall {n}, u n -> var -> e n -> e n    
 }.
 
 (***********************************************************************)
@@ -23,7 +63,8 @@ Class Subst (e : nat -> Set) (u : nat -> Set) `{Syntax e} `{Syntax u} := {
 (***********************************************************************)
 
 (* These are the general form of the lemmas in the Lemmas.v file. *)
-   
+
+(* Properties about operations in the `Syntax` class. *)   
 
 Class SyntaxTheory (exp : nat -> Set) `{H: Syntax exp} := {
 
@@ -48,6 +89,8 @@ Class SyntaxTheory (exp : nat -> Set) `{H: Syntax exp} := {
       fv (close x1 e1) [=] remove x1 (fv e1);
 }.
 
+(* Properties about the substitution operations (and their 
+   interaction with the operations in the Syntax class). *)
 
 Class SubstTheory (exp : nat -> Set) (u : nat -> Set) 
       `{H: Subst exp u} := {
@@ -104,8 +147,15 @@ Class SubstTheory (exp : nat -> Set) (u : nat -> Set)
                                                           
   }.
 
+(* Properties about the substitution operations that also 
+   refer to the free variable constructor for `u` terms.
+   We generalize this constructor as an additional parameter
+   to the type class.
+ *)
+
+
 Class SubstVarTheory (exp : nat -> Set) (u : nat -> Set) 
-      (uvar : forall {n}, atom -> u n) `{H: Subst exp u} := {
+      (uvar : forall {n}, var -> u n) `{H: Subst exp u} := {
 
     size_open_var : forall k (e : exp (S k)) x,
       size (open (uvar x) e) = size e;
@@ -127,6 +177,7 @@ Class SubstVarTheory (exp : nat -> Set) (u : nat -> Set)
         x1 <> x2 ->
         open (uvar x2) (subst (weaken e1) x1 e2) = 
           subst e1 x1 (open (uvar x2) e2);
+
    subst_close_open : forall n1 (e2 : exp (S n1)) e1 x1 x2,
       x2 `notin` fv e2 ->
       x2 `notin` fv e1 ->
@@ -135,10 +186,14 @@ Class SubstVarTheory (exp : nat -> Set) (u : nat -> Set)
       close x2 
        (subst e1 x1 (open (uvar x2) e2)); 
 
-   subst_intro  : forall n (e1 : exp (S n)) (x1:atom) (e2 : u n),
+   subst_intro  : forall n (e1 : exp (S n)) (x1:var) (e2 : u n),
       x1 `notin` fv e1 ->
       open e2 e1 = subst e2 x1 (open (uvar x1) e1) ;
 }.
+
+(* Properties about the substitution operation that 
+   require distributing substitutions to both `exp` terms 
+   and `u` terms. *)
 
 Class SubstSubstTheory (exp : nat -> Set) (u : nat -> Set) 
       `{H: Subst exp u}`{HU: Subst u u} := {
@@ -179,6 +234,11 @@ Create HintDb weaken.
 Create HintDb size.
 Create HintDb subst.
 
+(* The idea of this tactic is that each of the operations in 
+   the `Syntax` and `Subst` classes come with their own library
+   of rewriting hints. We can apply them all, repeatedly, using 
+   the following tactic. *)
+
 Ltac simp_syntax := repeat first [ 
                        simp subst
                      || simp open
@@ -186,6 +246,7 @@ Ltac simp_syntax := repeat first [
                      || simp weaken
                      || simp size
                      || simp fv
+                     || simp syntax
                      ].
 
 
@@ -198,8 +259,8 @@ Ltac simp_syntax := repeat first [
     expression or variable.  The following definition provides a
     convenient shorthand for such uses.  Note that the order of
     arguments is switched relative to the definition above.  For
-    example, [e ^ x] can be read as "substitute the variable [x]
-    for index [0] in [e]".
+    example, [e ^ fvar x] can be read as "substitute the free 
+    variable [x] for index [0] in [e]".
 *)
 
 Declare Scope syntax_scope.
