Stlc/ClassInstances.v
@@ -1,0 +1,76 @@
+Require Export Stlc.Classes.
+Require Import Stlc.DefinitionsSyntax.
+Require Import Stlc.Lemmas.
+
+(***********************************************************************)
+(** * Class  instances *)
+(***********************************************************************)
+
+#[global] Instance Syntax_exp : Syntax exp := { 
+    fv := fun {n} => @fv_exp n;
+    size := fun {n} => @size_exp n; 
+    weaken := fun {n} =>  @weaken_exp n;
+    close := fun {n} => @close_exp_wrt_exp n;
+}.
+
+#[global] Opaque Syntax_exp.
+
+#[global] Instance Subst_exp : Subst exp exp := {
+    open := fun {n} => @open_exp_wrt_exp n;
+    subst := fun {n} => @subst_exp_wrt_exp n
+}.
+#[global] Opaque Subst_exp.
+
+
+#[global] Instance STE :  SyntaxTheory exp := {
+  size_weaken := size_exp_weaken_exp;
+  fv_weaken := fv_exp_weaken_exp;
+  size_min  := size_exp_min;
+  size_close := size_exp_close_exp_wrt_exp;
+  close_inj := close_exp_wrt_exp_inj;
+  close_weaken := close_exp_wrt_exp_weaken_exp;
+  fv_close := fv_exp_close_exp_wrt_exp;
+}.
+
+
+#[global] Opaque STE.
+
+#[global] Instance SSTE : SubstTheory exp exp := {
+  size_open := size_exp_open_exp_wrt_exp;
+  open_weaken := open_exp_wrt_exp_weaken_exp;
+  fv_open_lower := fv_exp_open_exp_wrt_exp_lower;
+  fv_open_upper := fv_exp_open_exp_wrt_exp_upper; 
+  fv_subst_fresh := fv_exp_subst_exp_wrt_exp_fresh;
+  fv_subst_lower := fv_exp_subst_exp_wrt_exp_lower;
+  fv_subst_notin := fv_exp_subst_exp_wrt_exp_notin;
+  fv_subst_upper := fv_exp_subst_exp_wrt_exp_upper; 
+
+  subst_close := subst_exp_close_exp_wrt_exp;
+  subst_fresh_eq := subst_exp_wrt_exp_fresh_eq;
+  subst_fresh_same := subst_exp_wrt_exp_fresh_same;
+  subst_weaken := subst_exp_wrt_exp_weaken_exp;
+  subst_spec := subst_exp_wrt_exp_spec;
+}.
+
+
+#[global] Instance SVSTE :  SubstVarTheory exp exp (@var_f) := {
+  size_open_var := size_exp_open_exp_wrt_exp_var;
+  close_open := close_exp_wrt_exp_open_exp_wrt_exp;
+  open_close := open_exp_wrt_exp_close_exp_wrt_exp;
+  open_inj := open_exp_wrt_exp_inj;
+  subst_open_var := subst_exp_open_exp_wrt_exp_var;
+  subst_close_open := 
+    subst_exp_wrt_exp_close_exp_wrt_exp_open_exp_wrt_exp;
+  subst_intro := subst_exp_wrt_exp_intro;
+
+}.
+
+
+#[global] Opaque SVSTE.
+
+#[global] Instance SSSTE : SubstSubstTheory exp exp := {
+  subst_open := subst_exp_open_exp_wrt_exp;
+  subst_subst := subst_exp_wrt_exp_subst_exp_wrt_exp;
+}.
+
+#[global] Opaque SSSTE.
