Stlc/DefinitionsTyping.v
@@ -1,0 +1,109 @@
+(***********************************************************************)
+(** * Typing rules for STLC *)
+(***********************************************************************)
+
+(** This file containes definitions for the typing rules for a locally-nameless
+    representation of a Curry-Style simply-typed lambda calculus.
+*)
+
+
+Require Import Metalib.Metatheory.
+Require Import Metalib.LibLNgen.
+
+Require Import Utf8 Arith Compare_dec Lia.
+
+(* equations *)
+Set Warnings "-notation-overridden".
+Require Import Relation_Operators Program.
+Close Scope program_scope.
+From Equations Require Import Equations.
+
+Require Import Stlc.DefinitionsSyntax.
+Require Export Stlc.ClassInstances.
+Import SyntaxNotations.
+Open Scope syntax_scope.
+
+(***********************************************************************)
+(** * Typing contexts *)
+(***********************************************************************)
+
+(** We represent typing contexts as association lists (lists of pairs of
+    keys and values) whose keys are [atom]s.
+*)
+
+Definition ctx : Set := list (atom * typ).
+
+(** For STLC, contexts bind [atom]s to [typ]s.
+
+    Lists are defined in Coq's standard library, with the constructors
+    [nil] and [cons].  The list library includes the [::] notation for
+    cons as well as standard list operations such as append, map, and
+    fold. The infix operation [++] is list append.
+
+    The Metatheory library extends this reasoning by instantiating the
+    AssocList library to provide support for association lists whose keys
+    are [atom]s.  Everything in this library is polymorphic over the type
+    of objects bound in the environment.  Look in AssocList.v for
+    additional details about the functions and predicates that we mention
+    below.  *)
+
+
+(***********************************************************************)
+(** * Typing relation *)
+(***********************************************************************)
+
+(** The definition of the typing relation is straightforward.  In
+    order to ensure that the relation holds for only well-formed
+    environments, we check in the [typing_var] case that the
+    environment is [uniq].  The structure of typing derivations
+    implicitly ensures that the relation holds only for locally closed
+    expressions.
+
+    Finally, note the use of cofinite quantification in
+    the [typing_abs] case.
+*)
+
+Inductive typing : ctx -> exp 0 -> typ -> Prop :=
+ | typing_var : forall (G:ctx) (x:atom) (T:typ),
+     uniq G ->
+     binds x T G  ->
+     typing G (var_f x) T
+ | typing_abs : forall (L:vars) (G:ctx) (T1:typ) (e:exp 1) (T2:typ),
+     (forall x , x `notin` L -> typing ([(x,T1)] ++ G) (e ^ var_f x) T2)  ->
+     typing G (abs e) (typ_arrow T1 T2)
+ | typing_app : forall (G:ctx) (e1 e2:exp 0) (T2 T1:typ),
+     typing G e1 (typ_arrow T1 T2) ->
+     typing G e2 T1 ->
+     typing G (app e1 e2) T2 .
+
+Derive Signature for typing.
+
+(***********************************************************************)
+(** * Values and Small-step Evaluation *)
+(***********************************************************************)
+
+(** Finally, we define values and a call-by-name small-step evaluation
+    relation. In STLC, abstractions are the only value. *)
+
+Definition is_value (e : exp 0) : Prop :=
+  match e with
+  | abs _   => True
+  | _       => False
+  end.
+
+(** For [step_beta], note that we use [open_exp_wrt_exp] instead of
+    substitution --- no variable names are involved.
+
+    Note also the hypotheses in [step] that ensure that the relation holds
+    only for locally closed terms.  *)
+
+Inductive step : exp 0 -> exp 0 -> Prop :=
+ | step_beta : forall (e1:exp 1)(e2:exp 0),
+     step (app (abs e1) e2) (e1 ^ e2)
+ | step_app : forall (e1 e2 e1':exp 0),
+     step e1 e1' ->
+     step (app e1 e2) (app e1' e2).
+
+Derive Signature for step.
+
+#[global] Hint Constructors typing step : core.
