Stlc/Lemmas.v
@@ -16,19 +16,23 @@ Require Export Metalib.LibLNgen.
 Import Coq.Classes.RelationClasses.
 Require Import Lia.
 
-Require Import Stlc.Classes.
-Import SyntaxNotations.
-Open Scope syntax_scope.
+Require Import Stlc.DefinitionsSyntax.
 
-Require Export Stlc.Definitions.
+(* This file was originally produced by the LNgen tool. It has been modified to 
+   use the well-scoped expressions.
+*)
 
-(* Tactics for simplifying syntax definitions *)
+(* *********************************************************************** *)
+(** * Tactic support *)
+
+
+(* Simplify the equations versions of the functions. *)
 
 Ltac simp_stlc := repeat first [ 
                        simp subst_exp_wrt_exp
                      || simp open_exp_wrt_exp
                      || simp close_exp_wrt_exp
-                     || simp weaken_exp
+                     || simpl weaken_exp
                      || simpl size_exp
                      || simpl fv_exp
                      || simp increase_fin 
@@ -36,94 +40,17 @@ Ltac simp_stlc := repeat first [
                      || simp fin
                      ].
 
-Lemma fv_exp_var_b : forall n (m: fin n), fv (var_b m) = {}. 
-Proof. reflexivity. Qed.
-Lemma fv_exp_var_f : forall n (x:atom), fv (var_f (n:=n) x) = {{x}}.
-Proof. reflexivity. Qed.
-Lemma fv_exp_abs : forall n (e: exp (S n)), fv (abs e) = fv e.
-Proof. reflexivity. Qed.
-Lemma fv_exp_app : forall n (e1 : exp n) (e2: exp n), fv (app e1 e2) = fv e1 `union` fv e2.
-Proof. reflexivity. Qed.
+(* like an inversion tactic for equalities *)
+Ltac noconf_exp := 
+  match goal with 
+    | [ H : var_b _ = var_b _ |- _ ] => noconf H
+    | [ H : var_f _ = var_f _ |- _ ] => noconf H
+    | [ H : abs _ = abs _ |- _ ] => noconf H
+    | [ H : app _ _ = app _ _ |- _ ] => noconf H
+  end.
 
-#[export] Hint Rewrite fv_exp_var_b fv_exp_var_f fv_exp_abs fv_exp_app : fv.
-
-(* Re-define behavior of size in terms of size_exp *)
-Lemma size_exp_var_b : forall n (m: fin n), size (var_b m) = 1. 
-Proof. reflexivity. Qed.
-Lemma size_exp_var_f : forall n (x:atom), size (var_f (n:=n) x) = 1.
-Proof. reflexivity. Qed.
-Lemma size_exp_abs : forall n (e: exp (S n)), size (abs e) = 1 + (size e).
-Proof. reflexivity. Qed.
-Lemma size_exp_app : forall n (e1 : exp n) (e2: exp n), size (app e1 e2) = 1 + size e1 + size e2.
-Proof. reflexivity. Qed.
-
-#[export] Hint Rewrite size_exp_var_b size_exp_var_f size_exp_abs size_exp_app : size.
-
-Lemma weaken_exp_var_b : forall n (m: fin n),   weaken  (var_b m) = var_b (increase_fin m).
-Proof. reflexivity. Qed.
-Lemma weaken_exp_var_f : forall n (x:atom), weaken (var_f (n:=n) x) = var_f x.
-Proof. reflexivity. Qed.
-Lemma weaken_exp_abs : forall n (e: exp (S n)), weaken (abs e) = abs (weaken e).
-Proof. reflexivity. Qed.
-Lemma weaken_exp_app : forall n (e1 : exp n) (e2: exp n), weaken (app e1 e2) = app (weaken e1) (weaken e2).
-Proof. reflexivity. Qed.
-
-#[export] Hint Rewrite weaken_exp_var_b weaken_exp_var_f weaken_exp_abs weaken_exp_app : weaken.
-
-Lemma close_exp_var_b : forall n x (m: fin n),   close x (var_b m) = var_b (increase_fin m).
-Proof. reflexivity. Qed.
-Lemma close_exp_var_f : forall n (x1 x2:atom), close x1 (var_f (n:=n) x2) = if (x1 == x2) then (var_b (gof n)) else (var_f x2).
-Proof. reflexivity. Qed.
-Lemma close_exp_abs : forall n (e: exp (S n)) x1, close x1 (abs e) = abs (close x1 e).
-Proof. reflexivity. Qed.
-Lemma close_exp_app : forall n (e1 : exp n) (e2: exp n) x1, close x1 (app e1 e2) = app (close x1 e1) (close x1 e2).
-Proof. reflexivity. Qed.
-
-#[export] Hint Rewrite close_exp_var_b close_exp_var_f close_exp_abs close_exp_app : close.
-
-Lemma open_exp_var_b : forall n (u:exp n) (m: fin (S n)), 
-    open u (var_b m) = 
-      match decrease_fin n m with
-      | Some f => var_b f
-      | None => u
-      end.
-Proof. reflexivity. Qed.
-Lemma open_exp_var_f : forall n (u:exp n) (x:atom), open u (var_f (n:= S n) x) = var_f x.
-Proof. reflexivity. Qed.
-
-Lemma open_exp_abs : forall n (u:exp n) (e: exp (S (S n))), 
-    open u (abs e) = abs (open (weaken u) e).
-Proof. reflexivity. Qed. 
-Lemma open_exp_app : forall n (u:exp n) (e1 : exp (S n)) (e2: exp (S n)), 
-    open u (app e1 e2) = app (open u e1) (open u e2).
-Proof. reflexivity. Qed.
-
-#[export] Hint Rewrite open_exp_var_b open_exp_var_f open_exp_abs open_exp_app : open.
-
-Lemma subst_exp_var_b : forall n (u:exp n) (y:atom) (m: fin n), 
-    subst u y (var_b m) = var_b m.
-Proof. reflexivity. Qed.
-Lemma subst_exp_var_f : forall n (u:exp n) (y:atom) (x:atom), 
-    subst u y (var_f (n:=n) x) = if x == y then u else var_f x.
-Proof. reflexivity. Qed.
-Lemma subst_exp_abs : forall n (u:exp n) (y:atom) (e: exp (S n)), 
-    subst u y (abs e) = abs (subst (weaken u) y e).
-Proof. reflexivity. Qed.
-Lemma subst_exp_app : forall n (u:exp n) (y:atom) (e1 : exp n) (e2: exp n), 
-    subst u y (app e1 e2) = app (subst u y e1) (subst u y e2).
-Proof. reflexivity. Qed.
-
-#[export] Hint Rewrite subst_exp_var_b subst_exp_var_f subst_exp_abs subst_exp_app : subst.
-
-
-(* *********************************************************************** *)
-(** * Tactic support *)
 
 (** Additional hint declarations. *)
-
-(*
-#[global] Hint Resolve @plus_le_compat : lngen.
-*)
 
 (* Can't do this automatically b/c we need to have the 
    equality around. But then the option in the equality
@@ -150,7 +77,6 @@ Ltac default_case_split ::=
     | progress safe_f_equal
     ].
 
-
 (* *********************************************************************** *)
 (** * Theorems about [weaken] *)
 
@@ -162,7 +88,7 @@ Lemma size_exp_weaken_exp :
   size_exp (weaken_exp e1) = size_exp e1).
 Proof.
   intros n1 e1.
-  funelim (weaken_exp e1); program_simpl.
+  dependent induction e1; program_simpl.
 Qed.
 
 #[global] Hint Resolve size_exp_weaken_exp : lngen.
@@ -174,7 +100,7 @@ Lemma fv_exp_weaken_exp :
   fv_exp (weaken_exp e1) = fv_exp e1).
 Proof. 
   intros n1 e1.
-  funelim (weaken_exp e1); program_simpl.
+  dependent induction e1; program_simpl.
 Qed.
 
 #[global] Hint Resolve fv_exp_weaken_exp : lngen.
@@ -331,7 +257,7 @@ forall n1 (e2 : exp n1) e1,
   open_exp_wrt_exp e1 (weaken_exp e2) = e2.
 Proof.
 intros n1 e2.
-funelim (weaken_exp e2); default_simp.
+dependent induction e2; default_simp.
 Qed.
 #[global] Hint Resolve open_exp_wrt_exp_weaken_exp : lngen.
 #[export] Hint Rewrite open_exp_wrt_exp_weaken_exp using solve [auto] : lngen.
@@ -409,7 +335,7 @@ Lemma fv_exp_subst_exp_wrt_exp_notin :
 Proof.
 intros n1 e1.
 dependent induction e1; default_simp.
-eapply IHe1. auto. simp_stlc.
+eapply IHe1; default_simp. 
 Qed.
 
 #[global] Hint Resolve fv_exp_subst_exp_wrt_exp_notin : lngen.
@@ -445,7 +371,7 @@ intros n1 e2.
 dependent induction e2. 
 all: default_simp.
 specialize (IHe2 (weaken_exp e1)).
-eapply IHe2; simp_stlc; auto.
+eapply IHe2; default_simp. 
 Qed.
 
 
@@ -471,8 +397,7 @@ Lemma subst_exp_wrt_exp_fresh_same :
 Proof.
 intros n1 e2.
 dependent induction e2; default_simp.
-specialize (IHe2 (weaken_exp e1)).
-eapply IHe2. simp_stlc.
+eapply IHe2; default_simp.
 Qed.
 
 #[global] Hint Resolve subst_exp_wrt_exp_fresh_same : lngen.
@@ -494,8 +419,8 @@ Lemma subst_exp_wrt_exp_weaken_exp :
     weaken_exp (subst_exp_wrt_exp e1 x1 u) = 
     subst_exp_wrt_exp (weaken_exp e1) x1 (weaken_exp u).
 Proof.
-  intros.
-  funelim (weaken_exp u); simp_stlc; default_simp.
+  intros n e1 x1 u.
+  dependent induction u; default_simp.
 Qed.
 
 #[global] Hint Resolve subst_exp_wrt_exp_weaken_exp : lngen.
@@ -525,9 +450,7 @@ forall n1 (e2 : exp (S n1)) e1 x1 x2,
 Proof.
 intros; default_simp.
 rewrite subst_exp_open_exp_wrt_exp.
-f_equal.
-simp subst.
-destruct (x2 == x1) eqn:E. subst. fsetdec. auto.
+default_simp.
 Qed.
 
 #[global] Hint Resolve subst_exp_open_exp_wrt_exp_var : lngen.
@@ -578,7 +501,7 @@ symmetry. eauto using decrease_to_fin.
 specialize (IHe2 _ e2 ltac:(auto) ltac:(auto)).
 specialize (IHe2 (weaken_exp e1)).
 eapply IHe2; eauto.
-all: simp_stlc. 
+all: default_simp. 
 Qed.
 
 #[global] Hint Resolve subst_exp_wrt_exp_close_exp_wrt_exp_open_exp_wrt_exp : lngen.
@@ -614,56 +537,3 @@ Qed.
 
 Ltac default_auto ::= auto; tauto.
 Ltac default_autorewrite ::= fail.
-
-#[global] Instance STE :  SyntaxTheory exp := {
-  size_weaken := size_exp_weaken_exp;
-  fv_weaken := fv_exp_weaken_exp;
-  size_min  := size_exp_min;
-  size_close := size_exp_close_exp_wrt_exp;
-  close_inj := close_exp_wrt_exp_inj;
-  close_weaken := close_exp_wrt_exp_weaken_exp;
-  fv_close := fv_exp_close_exp_wrt_exp;
-}.
-
-
-#[global] Opaque STE.
-
-#[global] Instance SSTE : SubstTheory exp exp := {
-  size_open := size_exp_open_exp_wrt_exp;
-  open_weaken := open_exp_wrt_exp_weaken_exp;
-  fv_open_lower := fv_exp_open_exp_wrt_exp_lower;
-  fv_open_upper := fv_exp_open_exp_wrt_exp_upper; 
-  fv_subst_fresh := fv_exp_subst_exp_wrt_exp_fresh;
-  fv_subst_lower := fv_exp_subst_exp_wrt_exp_lower;
-  fv_subst_notin := fv_exp_subst_exp_wrt_exp_notin;
-  fv_subst_upper := fv_exp_subst_exp_wrt_exp_upper; 
-
-  subst_close := subst_exp_close_exp_wrt_exp;
-  subst_fresh_eq := subst_exp_wrt_exp_fresh_eq;
-  subst_fresh_same := subst_exp_wrt_exp_fresh_same;
-  subst_weaken := subst_exp_wrt_exp_weaken_exp;
-  subst_spec := subst_exp_wrt_exp_spec;
-}.
-
-
-#[global] Instance SVSTE :  SubstVarTheory exp exp (@var_f) := {
-  size_open_var := size_exp_open_exp_wrt_exp_var;
-  close_open := close_exp_wrt_exp_open_exp_wrt_exp;
-  open_close := open_exp_wrt_exp_close_exp_wrt_exp;
-  open_inj := open_exp_wrt_exp_inj;
-  subst_open_var := subst_exp_open_exp_wrt_exp_var;
-  subst_close_open := 
-    subst_exp_wrt_exp_close_exp_wrt_exp_open_exp_wrt_exp;
-  subst_intro := subst_exp_wrt_exp_intro;
-
-}.
-
-
-#[global] Opaque SVSTE.
-
-#[global] Instance SSSTE : SubstSubstTheory exp exp := {
-  subst_open := subst_exp_open_exp_wrt_exp;
-  subst_subst := subst_exp_wrt_exp_subst_exp_wrt_exp;
-}.
-
-#[global] Opaque SSSTE.
